Decider_Pipeline.v
@@ -1,0 +1,256 @@
+From BusyCoq Require Import BB52Statement.
+From BusyCoq Require Import ListTape.
+From BusyCoq Require Import Decider_RepWL.
+
+Definition halt_time_verifier(tm:TM Σ)(n:nat):bool :=
+  match ListES_Steps tm n {| l := nil; r := nil; m := Σ0; s := St0 |} with
+  | Some {| l:=_; r:=_; m:=m0; s:=s0 |} =>
+    match tm s0 m0 with
+    | None => true
+    | _ => false
+    end
+  | None => false
+  end.
+
+Lemma halt_time_verifier_spec tm n:
+  halt_time_verifier tm n = true ->
+  TM_CoqBB5.HaltsAt _ tm n (InitES Σ Σ0).
+Proof.
+  unfold halt_time_verifier,TM_CoqBB5.HaltsAt.
+  intro H.
+  pose proof (ListES_Steps_spec tm n {| l := nil; r := nil; m := Σ0; s := St0 |}).
+  destruct (ListES_Steps tm n {| l := nil; r := nil; m := Σ0; s := St0 |}).
+  2: cg.
+  rewrite ListES_toES_O in H0.
+  eexists.
+  split.
+  - apply H0.
+  - destruct l0 as [l0 r0 m0 s0].
+    cbn.
+    destruct (tm s0 m0); cg.
+Qed.
+
+Definition BB:N := 47176869.
+
+Fixpoint nat_eqb_N(n:nat)(m:N) :=
+match n,m with
+| O,N0 => true
+| S n0,Npos _ => nat_eqb_N n0 (N.pred m)
+| _,_ => false
+end.
+
+Lemma nat_eqb_N_spec n m :
+  nat_eqb_N n m = true -> n = N.to_nat m.
+Proof.
+  gd m.
+  induction n; intros.
+  - cbn in H.
+    destruct m0; cbn; cg.
+  - destruct m0.
+    + cbn in H. cg.
+    + cbn in H.
+      specialize (IHn (Pos.pred_N p) H). lia.
+Qed.
+
+
+Definition halt_decider_max := halt_decider 47176870.
+Lemma halt_decider_max_spec: HaltDecider_WF (N.to_nat BB) halt_decider_max.
+Proof.
+  eapply halt_decider_WF.
+  unfold BB.
+  replace (S (N.to_nat 47176869)) with (N.to_nat 47176870) by lia.
+  replace (Init.Nat.of_num_uint
+    (Number.UIntDecimal
+       (Decimal.D4
+          (Decimal.D7
+             (Decimal.D1
+                (Decimal.D7 (Decimal.D6 (Decimal.D8 (Decimal.D7 (Decimal.D0 Decimal.Nil))))))))))
+  with (N.to_nat 47176870).
+  1: apply Nat.le_refl.
+  symmetry.
+  apply nat_eqb_N_spec.
+  vm_compute.
+  reflexivity.
+Time Qed.
+
+Definition BB5_champion := (makeTM BR1 CL1 CR1 BR1 DR1 EL0 AL1 DL1 HR1 AL0).
+
+Lemma BB5_lower_bound:
+  exists tm,
+  TM_CoqBB5.HaltsAt _ tm (N.to_nat BB) (InitES Σ Σ0).
+Proof.
+  exists BB5_champion.
+  apply halt_time_verifier_spec.
+  vm_compute.
+  reflexivity.
+Time Qed.
+
+
+Definition decider0 := HaltDecider_nil.
+Definition decider1 := halt_decider 130.
+Definition decider2 := (loop1_decider 130 (1::2::4::8::16::32::64::128::256::512::nil)).
+
+Definition decider3 := (NGramCPS_decider_impl2 1 1 100).
+Definition decider4 := (NGramCPS_decider_impl2 2 2 200).
+Definition decider5 := (NGramCPS_decider_impl2 3 3 400).
+Definition decider6 := (NGramCPS_decider_impl1 2 2 2 1600).
+Definition decider7 := (NGramCPS_decider_impl1 2 3 3 1600).
+
+Definition decider8 := (loop1_decider 4100 (1::2::4::8::16::32::64::128::256::512::1024::2048::4096::nil)).
+
+Definition decider9 := (NGramCPS_decider_impl1 4 2 2 600).
+Definition decider10 := (NGramCPS_decider_impl1 4 3 3 1600).
+Definition decider11 := (NGramCPS_decider_impl1 6 2 2 3200).
+Definition decider12 := (NGramCPS_decider_impl1 6 3 3 3200).
+Definition decider13 := (NGramCPS_decider_impl1 8 2 2 1600).
+Definition decider14 := (NGramCPS_decider_impl1 8 3 3 1600).
+
+Lemma decider2_WF: HaltDecider_WF (N.to_nat BB) decider2.
+Proof.
+  apply loop1_decider_WF.
+  unfold BB.
+  lia.
+Qed.
+
+Lemma root_q_WF:
+  SearchQueue_WF (N.to_nat BB) root_q root.
+Proof.
+  apply SearchQueue_init_spec,root_WF.
+Qed.
+
+Definition root_q_upd1:=
+  (SearchQueue_upd root_q decider2).
+
+Lemma root_q_upd1_WF:
+  SearchQueue_WF (N.to_nat BB) root_q_upd1 root.
+Proof.
+  apply SearchQueue_upd_spec.
+  - apply root_q_WF.
+  - apply decider2_WF.
+Qed.
+
+Definition first_trans_is_R(x:TNF_Node):bool :=
+  match x.(TNF_tm) St0 Σ0 with
+  | Some {| nxt:=_; dir:=Dpos; out:=_ |} => true
+  | _ => false
+  end.
+
+Definition root_q_upd1_simplified:SearchQueue:=
+  (filter first_trans_is_R (fst root_q_upd1), nil).
+
+Lemma TM_rev_upd'_TM0 s0 o0:
+  (TM_upd' (TM0) St0 Σ0 (Some {| nxt := s0; dir := Dneg; out := o0 |})) =
+  (TM_rev Σ (TM_upd' (TM0) St0 Σ0 (Some {| nxt := s0; dir := Dpos; out := o0 |}))).
+Proof.
+  repeat rewrite TM_upd'_spec.
+  fext. fext.
+  unfold TM_upd,TM_rev,TM0.
+  St_eq_dec x St0.
+  - Σ_eq_dec x0 Σ0; cbn; reflexivity.
+  - cbn; reflexivity.
+Qed.
+
+Lemma root_q_upd1_simplified_WF:
+  SearchQueue_WF (N.to_nat BB) root_q_upd1_simplified root.
+Proof.
+  pose proof (root_q_upd1_WF).
+  cbn in H.
+  destruct H as [Ha Hb].
+  cbn.
+  split.
+  - intros x H0.
+    pose proof (Ha x). tauto.
+  - intro H0. apply Hb.
+    intros x H1.
+    destruct H1 as [H1|[H1|[H1|[H1|[H1|[H1|[H1|[H1|H1]]]]]]]]; try (specialize (H0 x); tauto).
+    1,2,3,4:
+      clear Ha; clear Hb;
+      destruct x as [tm cnt ptr];
+      cbn; invst H1;
+      rewrite TM_rev_upd'_TM0;
+      eapply HaltTimeUpperBound_LE_rev_InitES.
+    1: eassert (H2:_) by (apply (H0 {|
+             TNF_tm := TM_upd' (TM0) St0 Σ0 (Some {| nxt := St0; dir := Dpos; out := Σ0 |});
+             TNF_cnt := 9;
+             TNF_ptr := St1
+           |}); tauto); apply H2.
+    1: eassert (H2:_) by (apply (H0 {|
+             TNF_tm := TM_upd' (TM0) St0 Σ0 (Some {| nxt := St0; dir := Dpos; out := Σ1 |});
+             TNF_cnt := 9;
+             TNF_ptr := St1
+           |}); tauto); apply H2.
+    1: eassert (H2:_) by (apply (H0 {|
+             TNF_tm := TM_upd' (TM0) St0 Σ0 (Some {| nxt := St1; dir := Dpos; out := Σ0 |});
+             TNF_cnt := 9;
+             TNF_ptr := St2
+           |}); tauto); apply H2.
+    1: eassert (H2:_) by (apply (H0 {|
+             TNF_tm := TM_upd' (TM0) St0 Σ0 (Some {| nxt := St1; dir := Dpos; out := Σ1 |});
+             TNF_cnt := 9;
+             TNF_ptr := St2
+           |}); tauto); apply H2.
+Qed.
+
+Fixpoint length_tailrec0{T}(ls:list T)(n:N):N :=
+match ls with
+| nil => n
+| h::t => length_tailrec0 t (N.succ n)
+end.
+Definition length_tailrec{T}(ls:list T):N := length_tailrec0 ls 0.
+
+
+Inductive DeciderType :=
+| NG(hlen len:nat)
+| NG_LRU(len:nat)
+| RWL(len m:nat)
+| DNV(n:nat)(f:nat->Σ->nat)
+| WA(max_d:BinNums.Z)(n_l:nat)(f_l:nat->Σ->(nat*BinNums.Z))(n_r:nat)(f_r:nat->Σ->(nat*BinNums.Z))
+| Ha
+| Lp1
+| Holdout.
+
+
+Definition getDecider(x:DeciderType) :=
+match x with
+| NG hlen len =>
+  match hlen with
+  | O => NGramCPS_decider_impl2 len len 5000001
+  | _ => NGramCPS_decider_impl1 hlen len len 5000001
+  end
+| NG_LRU len =>
+  NGramCPS_LRU_decider len len 5000001
+| RWL len mnc => RepWL_ES_decider len mnc 320 150001
+| DNV n f => dfa_nfa_verifier n f
+| WA max_d n_l f_l n_r f_r => MITM_WDFA_verifier max_d n_l f_l n_r f_r 10000000
+| Ha => halt_decider_max
+| Lp1 => loop1_decider 1050000 (4096::8192::16384::32768::65536::131072::262144::524288::nil)
+| Holdout => holdout_checker
+end.
+
+Lemma getDecider_spec x:
+  HaltDecider_WF (N.to_nat BB) (getDecider x).
+Proof.
+  destruct x; unfold getDecider.
+  - destruct hlen.
+    + apply NGramCPS_decider_impl2_spec.
+    + apply NGramCPS_decider_impl1_spec.
+  - apply NGramCPS_LRU_decider_spec.
+  - apply RepWL_ES_decider_spec.
+  - apply dfa_nfa_verifier_spec.
+  - apply MITM_WDFA_verifier_spec.
+  - apply halt_decider_max_spec.
+  - apply loop1_decider_WF.
+    unfold BB.
+    replace (Init.Nat.of_num_uint
+  (Number.UIntDecimal
+     (Decimal.D1
+        (Decimal.D0
+           (Decimal.D5 (Decimal.D0 (Decimal.D0 (Decimal.D0 (Decimal.D0 Decimal.Nil))))))))) with
+    (N.to_nat 1050000).
+    1: lia.
+    symmetry.
+    apply nat_eqb_N_spec.
+    vm_compute.
+    reflexivity.
+  - apply holdout_checker_spec.
+Qed.
