Decider_RepWL.v
@@ -1,6 +1,16 @@
-Module MacroMachine.
+Require Import Lia.
+Require Import List.
+Require Import ZArith.
+Require Import FSets.FMapPositive.
 
-Require Import ListTape.
+From BusyCoq Require Import CustomTactics.
+From BusyCoq Require Import Encodings.
+From BusyCoq Require Import BB52Statement.
+From BusyCoq Require Import Prelims.
+From BusyCoq Require Import TM_CoqBB5.
+From BusyCoq Require Import ListTape.
+From BusyCoq Require Import TNF.
+From BusyCoq Require Import Decider_NGramCPS.
 
 Section MacroMachine_secion.
 
