TNF.v
@@ -527,3 +527,8 @@ Qed.
 Definition root_q := SearchQueue_init root.
 
 End TNF.
+
+Definition TNF_Node_list_to_N_list := map (fun (x:TNF_Node) => TM_to_N (TNF_tm x)).
+
+
+Compute (TM_to_N (makeTM BR1 HR1 CL0 ER0 DL0 CL1 AR1 BR0 DR0 DR1)).
